Update botworld state representation again
New design due to Jack. Robots no longer have names attached to them,
but (unique) names are used to refer to robots within squares and
events. Everything is much more local than previously.

botworld_propsTheory not updated yet.

botworldScript.sml
@@ -8,6 +8,9 @@ val _ = temp_tight_equality();
 
 val _ = new_theory"botworld"
 
+val _ = Parse.bring_to_front_overload","{Name=",",Thy="pair"};
+val _ = Parse.type_abbrev("state",``:botworld_data$state``);
+
 (* Port of Botworld to more idiomatic HOL *)
 
 val neighbour_coords_def = Define`
@@ -29,45 +32,41 @@ val neighbours_def = Define`
 
 (* environment phase *)
 
+val requests_def = Define`
+  requests i items r =
+    case r.command of
+    | Lift li => li = i ∧ canLift r (EL i items)
+    | Build is m => MEM i is ∧
+                    EVERY (λi. i < LENGTH items) is ∧
+                    IS_SOME (construct (MAP (λi. EL i items) is) m)
+    | _ => F`;
+
 val contested_def = Define`
   contested sq i ⇔
     i < LENGTH sq.items ∧
-    1 < LENGTH
-        (FILTER (λr. case r.command of
-                     | Lift li => li = i ∧ canLift r (EL i sq.items)
-                     | Build is m => MEM i is ∧
-                                     EVERY (λi. i < LENGTH sq.items) is ∧
-                                     IS_SOME (construct (MAP (λi. EL i sq.items) is) m)
-                     | _ => F)
-         sq.robots)`;
+    1 < LENGTH (FILTER (requests i sq.items) (MAP SND sq.robots))`;
 
 val fled_def = Define`
   (fled nb (Move dir) ⇔ dir < LENGTH nb ∧ IS_SOME (EL dir nb)) ∧
   (fled nb _ = F)`;
 
 val inspectAttempts_def = Define`
-  inspectAttempts intents i =
-    LENGTH (FILTER ($= (Inspect i)) intents)`;
+  inspectAttempts intents nm =
+    LENGTH (FILTER ($= (Inspect nm)) intents)`;
 
 val inspectShielded_def = Define`
-  inspectShielded robots r ⇔
-    inspectAttempts (MAP robot_command robots) r.name ≤
-    LENGTH (FILTER isInspectShield r.inventory)`;
+  inspectShielded intents nm inventory ⇔
+    inspectAttempts intents nm ≤
+    LENGTH (FILTER isInspectShield inventory)`;
 
 val destroyAttempts_def = Define`
-  destroyAttempts intents i =
-    LENGTH (FILTER ($= (Destroy i)) intents)`;
+  destroyAttempts intents nm =
+    LENGTH (FILTER ($= (Destroy nm)) intents)`;
 
 val destroyShielded_def = Define`
-  destroyShielded robots r ⇔
-    destroyAttempts (MAP robot_command robots) r.name ≤
-    LENGTH (FILTER isDestroyShield r.inventory)`;
-
-val findRobotInSquare_def = Define`
-  findRobotInSquare n ls = case FILTER ($= n o robot_name) ls of
-                            | [] => NONE
-                            | (r::_) => SOME r
-`
+  destroyShielded intents nm inventory ⇔
+    destroyAttempts intents nm ≤
+    LENGTH (FILTER isDestroyShield inventory)`;
 
 val act_def = Define`
   act sq nb r =
@@ -86,22 +85,24 @@ val act_def = Define`
       if i < LENGTH r.inventory then
         Dropped i
       else Invalid
-    | Inspect i =>
-      (case findRobotInSquare i sq.robots of
+    | Inspect nm =>
+      (case ALOOKUP sq.robots nm of
           NONE => Invalid
         | SOME r' => if ¬fled nb r'.command then
-                       if ¬inspectShielded sq.robots r' then
-                         Inspected r'
-                       else InspectBlocked i
-                     else InspectTargetFled i)
-    | Destroy i =>
-      (case findRobotInSquare i sq.robots of
+                       if ¬inspectShielded
+                           (MAP (robot_command o SND) sq.robots) nm r'.inventory
+                       then Inspected nm r'
+                       else InspectBlocked nm
+                     else InspectTargetFled nm)
+    | Destroy nm =>
+      (case ALOOKUP sq.robots nm of
           NONE    => Invalid
         | SOME r' => if ¬fled nb r'.command then
-                         if ¬destroyShielded sq.robots r' then
-                             Destroyed i
-                         else DestroyBlocked i
-                     else DestroyTargetFled i)
+                         if ¬destroyShielded
+                             (MAP (robot_command o SND) sq.robots) nm r'.inventory
+                         then Destroyed nm
+                         else DestroyBlocked nm
+                     else DestroyTargetFled nm)
     | Build is m =>
       if EVERY (λi. i < LENGTH sq.items) is then
         if ¬EXISTS (contested sq) is then
@@ -114,59 +115,60 @@ val act_def = Define`
 
 val localActions_def = Define`
   localActions sq nb =
-    MAP (act sq nb) sq.robots`;
+    MAP (λ(nm,r). (nm, (r, act sq nb r))) sq.robots`;
 
 val defend_def = Define`
-  defend intents i =
-    dropN (destroyAttempts intents i) isDestroyShield o
-    dropN (inspectAttempts intents i) isInspectShield`;
+  defend intents nm =
+    dropN (destroyAttempts intents nm) isDestroyShield o
+    dropN (inspectAttempts intents nm) isInspectShield`;
 
 val updateInventory_def = Define`
-  updateInventory sq r a =
-    let intents = MAP robot_command sq.robots in
-    case a of
-    | MovedOut _ => r
-    | Lifted n => r with inventory := (EL n sq.items)::(defend intents r.name r.inventory)
-    | Dropped n => r with inventory := (defend intents r.name (remove_indices ($= n) 0 r.inventory))
-    | _ => r with inventory := defend intents r.name r.inventory`;
+  updateInventory sq nm (r,a) =
+    let intents = MAP (robot_command o SND) sq.robots in
+    (nm,
+      case a of
+      | MovedOut _ => r
+      | Lifted n => r with inventory := (EL n sq.items)::(defend intents nm r.inventory)
+      | Dropped n => r with inventory := (defend intents nm (remove_indices ($= n) 0 r.inventory))
+      | _ => r with inventory := defend intents nm r.inventory)`;
 
 val incomingFrom_def = Define`
   (incomingFrom dir NONE = []) ∧
   (incomingFrom dir (SOME sq) =
-   FLAT (MAP (λr. if r.command = Move (opposite dir) then [(r,MovedIn dir)] else []) sq.robots))`;
+   MAP (λ(nm,r). (nm, (r, MovedIn dir)))
+     (FILTER (λ(nm,r). r.command = Move (opposite dir)) sq.robots))`;
+
+val dropItem_def = Define`
+  dropItem (r,a) =
+    case a of Dropped i => [EL i r.inventory] | _ => []`;
+
+val usedItem_def = Define`
+  usedItem actions i =
+    EXISTS (λa. case a of Lifted l => i = l
+                | Built is _ => MEM i is
+                | _ => F) actions`;
 
 val event_def = Define`
   event sq nb =
-    let actions = localActions sq nb in
-    let veterans = MAP (UNCURRY (updateInventory sq)) (ZIP(sq.robots,actions)) in
-    let fallen = FLAT (MAP (λr. if MEM (Destroyed r.name) actions then
-                                      [<|components := shatter r
-                                        ;possessions := r.inventory|>]
-                                    else []) veterans) in
+    let oldRobotsActions = localActions sq nb in
+    let veterans = MAP (UNCURRY (updateInventory sq)) oldRobotsActions in
+    let actions = MAP (SND o SND) oldRobotsActions in
     <| robotActions :=
-       let immigrations = FLAT (GENLIST (λi. incomingFrom i (EL i nb)) (LENGTH nb)) in
-       let children = FLAT (MAP (λa. case a of Built _ r => [r] | _ => []) actions) in
-       ZIP (veterans,actions) ++ immigrations ++
-       ZIP (children, REPLICATE (LENGTH children) Created)
-     ; untouchedItems :=
-       remove_indices
-         (λi. EXISTS (λa. case a of Lifted l => i = l
-                                  | Built is _ => MEM i is
-                                  | _ => F)
-              actions)
-         0 sq.items
-     ; droppedItems :=
-       FLAT
-         (MAP (λ(r,a). case a of Dropped i => [EL i r.inventory]
-                               | _ => [])
-              (ZIP(sq.robots,actions)))
-     ; fallenItems := fallen
+       let immigrations = FLAT (GENLIST (λdir. incomingFrom dir (EL dir nb)) (LENGTH nb)) in
+       MAP2 (λ(nm,r) a. (nm,(r,a))) veterans actions ++ immigrations
+     ; createdRobots :=  MAP (SND o destBuilt) (FILTER isBuilt actions)
+     ; untouchedItems := remove_indices (usedItem actions) 0 sq.items
+     ; droppedItems := FLAT (MAP (dropItem o SND) oldRobotsActions)
+     ; fallenItems :=
+         MAP (λ(nm,r). <|components := shatter r
+                        ;possessions := r.inventory|>)
+             (FILTER (λ(nm,r). MEM (Destroyed nm) actions) veterans)
      |>`;
 
 (* computation phase *)
 
 val private_def = Define`
-  (private (Inspected r) = pInspected r.processor r.memory) ∧
+  (private (Inspected _ r) = pInspected r.processor r.memory) ∧
   (private Invalid = pInvalid) ∧
   (private _ = pNothing)`;
 
@@ -179,7 +181,7 @@ val ffi_from_observation_def = Define`
   define this in botworld_preambleTheory, as the environment produced by
   the translator (plus extra definitions as necessary) *)
 val preamble_env_def = Define`
-  preamble_env (ffi:'ffi ffi_state) = ARB:('ffi state # v environment)`;
+  preamble_env (ffi:'ffi ffi_state) = ARB:('ffi semanticPrimitives$state # v environment)`;
 
 val run_policy_def = Define`
   run_policy policy clock obs =
@@ -191,19 +193,24 @@ val run_policy_def = Define`
 val runMachine_def = Define`
   runMachine (obs,r) =
     let (command,prog) = run_policy r.memory r.processor obs in
-    r with <| command := command; memory := prog |>`;
+    (FST obs, r with <| command := command; memory := prog |>)`;
 
 val prepare_def = Define`
-  prepare ev (r,a) = ((r.name, ev, private a), r)
+  prepare ev (nm,(r,a)) = ((nm, ev, private a), r)
 `
 
 val computeSquare_def = Define`
-  computeSquare ev =
+  computeSquare t (c,ev) =
     <| items :=
          ev.untouchedItems ++ ev.droppedItems ++
          FLAT (MAP (λc. c.components ++ c.possessions) ev.fallenItems)
      ; robots :=
-         let ls = FILTER (λ(r,a). ¬isMovedOut a ∧ ¬MEM (Destroyed r.name) (MAP SND ev.robotActions)) ev.robotActions in
+         let ls =
+             FILTER (λ(nm,(r,a)). ¬isMovedOut a ∧ ¬MEM (Destroyed nm) (MAP (SND o SND) ev.robotActions))
+                    ev.robotActions ++
+             GENLIST (λi. (<| built_step := t; built_coord := c; id := i |>,
+                           (EL i ev.createdRobots, Passed)))
+                     (LENGTH ev.createdRobots) in
            MAP (runMachine o prepare ev) ls
      |>`;
 
@@ -213,61 +220,40 @@ val computeEvents_def = Define`
   computeEvents (g:grid) =
     FMAP_MAP2 (λ(c,sq). event sq (neighbours g c)) g`;
 
-val nameSquare_def = Define`
-  nameSquare num rs =
-     FOLDR (λr (num,rs). if r.name = 0 then (num + 1, (r with name := num) :: rs) else (num,r::rs))
-       (num,[]) rs`
-
-val robotNames_def = Define`
-  robotNames = MAP robot_name o square_robots
-`
-
-val allCoords_def = Define`
-  allCoords (f:coordinate |-> α) = QSORT ($< LEX $<) (SET_TO_LIST (FDOM f))`
-
-val allNames_def = Define`
-  allNames f = FLAT (MAP (robotNames o FAPPLY f) (allCoords f))`
-
-val maxList_def = Define`
-  maxList = FOLDL MAX 0
-`
-
-val mapRobotsInSquare_def = Define`
-  mapRobotsInSquare f sq = sq with robots updated_by MAP f
-`
-
-val mapRobots_def = Define`
-  mapRobots f = FMAP_MAP2 (mapRobotsInSquare f o SND)
-`
-
-val mkNames_def = Define`
-  mkNames g = let nextName = 1 + maxList (allNames g) in
-              SND (ITSET (λc (n,m). let sq = g ' c in
-                                    let (n',r') = nameSquare n sq.robots in
-                                    (n', m |+ (c,sq with robots := r')))
-                         (FDOM g) (nextName,FEMPTY))
-`
-
 val step_def = Define`
-  step g = mkNames (computeSquare o_f (computeEvents g))`;
+  step st =
+    <| grid := FMAP_MAP2 (computeSquare st.time_step) (computeEvents st.grid)
+     ; time_step := st.time_step + 1 |>`;
 
 val wf_state_def = Define`
-  wf_state g ⇔ ALL_DISTINCT (allNames g) ∧ EVERY ($< 0) (allNames g)
-`
+  wf_state st ⇔
+    ∀c1 c2 s1 s2.
+      FLOOKUP st.grid c1 = SOME s1 ∧
+      FLOOKUP st.grid c2 = SOME s2 ∧
+      c1 ≠ c2
+      ⇒
+      DISJOINT (set (MAP FST s1.robots)) (set (MAP FST s2.robots))`;
 
 val _ = Datatype`
-  state_with_hole = <| state : grid
-                     ; focal_name : num
+  state_with_hole = <| state : state
+                     ; focal_name : name
                      |>`;
 
 val wf_state_with_hole_def = Define`
   wf_state_with_hole s ⇔
-    wf_state s.state ∧ MEM s.focal_name (allNames s.state)
-`
+    wf_state s.state ∧
+    ∃sq.
+      sq ∈ FRANGE s.state.grid ∧
+      MEM s.focal_name (MAP FST sq.robots)`;
+
+val if_focal_def = Define`
+  if_focal fnm f (nm, r) = (nm, if nm = fnm then f r else r)`
 
 val fill_def = Define`
-  fill f s = mapRobots (λr. if r.name = s.focal_name then f r else r) s.state
-`;
+  fill f s =
+  s.state with grid updated_by $o_f
+    (λsq. sq with robots updated_by
+          MAP (if_focal s.focal_name f))`;
 
 val _ = overload_on("with_policy",``λc p.  robot_memory_fupd (K p) o robot_command_fupd (K c)``);
 val _ = overload_on("with_memory", ``λp. memory_fupd (K p)``)
@@ -278,22 +264,22 @@ val _ = overload_on("fill_with",``λp. fill (UNCURRY with_policy p)``);
 val steph_def = Define`
   steph command s =
     let s' = fill (robot_command_fupd (K command)) s in
-    let events = computeEvents s' in
+    let events = computeEvents s'.grid in
     if FEVERY (λ (_,ev).
                EVERY (λa. a ≠ Destroyed s.focal_name ∧
-                      ∀r. r.name = s.focal_name ⇒ a ≠ Inspected r)
-              (MAP SND ev.robotActions)) events
+                          ∀r. a ≠ Inspected s.focal_name r)
+              (MAP (SND o SND) ev.robotActions)) events
     then
-      let (ev,a) = CHOICE { (ev,a) | ∃r. MEM (r,a) ev.robotActions ∧ r.name = s.focal_name ∧ ev ∈ FRANGE events } in
+      let (ev,a) = CHOICE { (ev,a) | ∃r. MEM (s.focal_name,(r,a)) ev.robotActions ∧ ev ∈ FRANGE events } in
       SOME ((s.focal_name, ev, private a), s with state := step s')
     else NONE
 `;
 
 (* histories *)
 
-val _ = Parse.type_abbrev("history",``:grid llist``);
+val _ = Parse.type_abbrev("history",``:state llist``);
 
 val hist_def = Define`
-  hist s = LUNFOLD (λs. SOME (step s,s)) s`;
+  (hist:state->history) s = LUNFOLD (λs. SOME (step s,s)) s`;
 
 val _ = export_theory()
